
%% 8
\section{ Y Combinator. }

% https://mvanier.livejournal.com/2897.html

% See also http://r6.ca/blog/20060919T084800Z.html

$$
Y = λf.(λx.f(xx))(λx.f(xx))
$$

\begin{align*} 
Y\ g &= (λx.g(xx))(λx.g(xx)) \\
     &= g ((λx.g(xx)) (λx.g(xx))) \\
     &= g (Y\ g) \\
     &= g (g (g (g (g \ldots))))
\end{align*} 
and it never ends if we use it like that. Still, if we take (using Haskell notation)
\begin{minted}{haskell}
g h x | x == 1    = 1
      | otherwise = x * (h $ x - 1)
\end{minted}
then for example 
\begin{align*} 
Y\ g\ 4 &= g\ (Y\ g)\ 4                \\
        &= 4 * ((Y\ g)\ 3)             \\
        &= 4 * (g\ (Y\ g)\ 3)          \\
        &= 4 * 3 * ((Y\ g)\ 2)         \\
        &= 4 * 3 * (g\ (Y\ g)\ 2)      \\
        &= 4 * 3 * 2 * ((Y\ g)\ 1)     \\
        &= 4 * 3 * 2 * (g\ (Y\ g)\ 1)  \\
        &= 4 * 3 * 2 * 1               \\
        &= 24,\text{ also known as } 4!
\end{align*} 

Here, we have a definition of a recursive function (factorial) in a language that does
not directly allow recursion. Of course, that requires lazy evaluation ---
and the definitions for naturals and multiplication.
